Util.v
@@ -1,5 +1,6 @@
 Require Import Coq.Lists.List.
 Require Export Coq.Program.Equality.
+Export ListNotations.
 
 (* Decision procedure for nat equality, and some theorems about it. *)
 Theorem eq_nat_dec : forall (n m : nat), {n = m} + {n <> m}.
@@ -96,3 +97,30 @@ Hint Resolve f_equal : l3.
 (* Specialised versions of auto *)
 Ltac boom := auto with l3.
 Ltac eboom := eauto with l3.
+
+(* A [repeat] function on lists, and lemmas about it *)
+Fixpoint repeat {A} (n : nat) (e : A) : list A :=
+  match n with
+  | 0 => []
+  | S n' => e :: repeat n' e
+  end.
+
+Lemma repeat_length : forall A n (e : A),
+  length (repeat n e) = n.
+Proof with (simpl; auto).
+  intros.
+  induction n as [|n']...
+Qed.
+
+Lemma repeat_app : forall A n (e : A),
+  repeat (S n) e = repeat n e ++ [e].
+Proof.
+  intros.
+  induction n as [|n'].
+  Case "n = 0". auto.
+  Case "n = S n'".
+    replace (repeat (S (S n')) e) with (e :: repeat (S n') e).
+    rewrite IHn' at 1.
+    auto.
+    auto.
+Qed.
